IsoGraph.lean
@@ -13,6 +13,7 @@ import IsoGraph.Jump
 import IsoGraph.Leaves
 import IsoGraph.Dominate
 import IsoGraph.Branch
+import IsoGraph.Optimal
 import IsoGraph.Basic
 import IsoGraph.Invariants
 import IsoGraph.Constructions
